\setcounter{section}{4}
\section{U-Substitution (undoes chain rule)}

\ex{}{
    $$\int 2x\sqrt{1+x^2}dx$$
    Indentify $u$
    $$u = 1+x^2$$
    Find $du$
    $$du = 2x dx$$   
    Substitute with $u$
    $$\int u^\frac{1}{2}du$$
    Undo power rule
    $$\frac{2}{3}u^{\frac{3}{2}}$$
    Backsubstitute
    $$\frac{2}{3}\left(1+x^2\right)^{\frac{3}{2}}+c$$
}
\ex{}{
    $$\int x^3\cos(x^4+2)dx$$
    $$u=x^4+2$$
    $$du=4x^3dx$$
    $$\frac{1}{4}du=x^3dx$$
    You can move constants out front when you substitute
    $$\frac{1}{4}\int \cos u du$$
    $$\frac{1}{4}\sin u$$
    $$\frac{1}{4}\sin\left(1+x^2\right)+c$$
}

\ex{}{
    $$\int \sqrt{2x+1}dx$$
    $$u=2x+1$$
    $$du=2dx$$
    $$\frac{1}{2}du=dx$$
    $$\frac{1}{2}\int u^\frac{1}{2}du$$
    $$\frac{1}{2}\frac{2}{3}u^{\frac{3}{2}}$$
    $$\frac{1}{3}\left(2x+1\right)^{\frac{3}{2}}+c$$
}

\ex{}{
    $$\int \frac{x}{\sqrt{1-4x^2}}dx$$
    $$u=1-4x^2$$
    $$du=-8xdx$$
    $$-\frac{1}{8}du=xdx$$
    $$-\frac{1}{8}\int u^{-\frac{1}{2}}du$$
    $$-\frac{1}{8}2u^{\frac{1}{2}}$$
    $$-\frac{1}{4}\left(1-4x^2\right)^{\frac{1}{2}}+c$$
}

\ex{}{
    $$\int \cos 5xdx$$
    $$u = 5x$$
    $$du=5dx$$
    $$\frac{1}{5}du=dx$$
    $$\frac{1}{5}\int \cos(u)du$$
    $$\frac{1}{5}\sin(u)$$
    $$\frac{1}{5}\sin\left(5x\right)+c$$
}

\ex{}{
    $$\int x^5\sqrt{1+x^2}dx$$
    $$u=1+x^2 \to u-1=x^2$$
    $$x^4 = \left(u-1\right)^2$$
    $$du=2xdx$$
    $$\frac{1}{2}du=xdx$$
    We have $x\cdot x^4$ so that we can substitute, but we're left with $x^4$. We can rearrange the equation for $u$ to solve for $x^4$
    $$\frac{1}{2}\int u^{\frac{1}{2}}du x^4$$
    $$\frac{1}{2}\int u^{\frac{1}{2}}du (u-1)^2$$
    $$\frac{1}{2}\int u^{\frac{1}{2}}\left(u^2-2u+1\right)du$$
    $$\frac{1}{2}\int \left(u^{\frac{5}{2}}-2u^{\frac{3}{2}}+u^{\frac{1}{2}}\right)du$$
    $$\frac{1}{2}\left(\frac{2}{7}u^{\frac{7}{2}}-2\frac{2}{5}u^{\frac{5}{2}}+\frac{2}{3}u^{\frac{3}{2}}\right)$$
    $$\frac{1}{7}\left(1+x^2\right)^{\frac{7}{2}}-\frac{2}{5}\left(1+x^2\right)^{\frac{5}{2}}+\frac{1}{3}\left(1+x^2\right)^{\frac{3}{2}}+c$$
    
}

\qs{Question 29}{
    $$\int \frac{x}{\sqrt[4]{x+2}}dx$$
    $$u=x+2$$
    $$x=u-2$$
    $$du=dx$$
    $$\int u^{-\frac{1}{4}}(u-2)du = \int \left(u^{\frac{3}{4}}-2u^{-\frac{1}{4}}\right)du$$
    $$\frac{4}{7}u^{\frac{7}{4}}-2\frac{4}{3}u^{\frac{3}{4}}$$
    $$\frac{4}{7}\left(x+2\right)^{\frac{7}{4}}-\frac{8}{3}\left(x+2\right)^{\frac{3}{4}}+c$$
}

\qs{Question 25}{
    $$\int \sec^3 x \tan x dx$$
    \begin{center}
        \begin{tabular}{||c c||}
            \hline
            $y$ & $y'$ \\ [0.5ex]
            \hline\hline
            $\tan(x)$ & $\sec^2(x)$ \\
            \hline
            $\sec(x)$ & $\sec(x)\tan(x)$ \\ [1ex]
            \hline
        \end{tabular}
    \end{center}
    $$\int \sec^2 x \sec x \tan x dx$$
    $$u = \sec x$$
    $$du = \sec x \tan x dx$$
    $$\int u^2du=\frac{1}{3}u^3$$
    $$\frac{1}{3}\sec^3x+c$$
}

\qs{Question 17}{
    $$\int \frac{\cos \sqrt{t}}{\sqrt{t}}dt$$
    $$u=\sqrt{t}=t^{\frac{1}{2}}$$
    $$du=\frac{1}{2}t^{-\frac{1}{2}}dt$$
    $$2du=t^{-\frac{1}{2}}dt$$
    $$2\int \cos u du$$
    $$2\sin u$$
    $$2\sin\left(\sqrt{t}\right)+c$$
}

\qs{}{
    \begin{center}
        \begin{tabular}{||c c||}
            \hline
            $y$ & $y'$ \\ [0.5ex]
            \hline\hline
            $\tan(x)$ & $\sec^2(x)$ \\
            \hline
            $\sec(x)$ & $\sec(x)\tan(x)$ \\ [1ex]
            \hline
        \end{tabular}
    \end{center}
    $$\int^{\frac{\pi}{6}}_{-\frac{\pi}{6}} \tan^3 \theta d\theta$$
    $$=\int \tan \theta \tan^2 \theta d\theta$$
    \nt{
        $$\frac{\sin^2 x}{\cos^2 x}+\frac{\cos^2 x}{\cos^2 x} = \frac{1}{\cos^2 x}$$
        $$\tan^2 x + 1 = \sec^2 x$$
        $$\tan^2 x = \sec^2 x - 1$$
    }

    $$\int \tan \theta\left(\sec^2 \theta - 1\right)d\theta$$

    Distribute

    $$=\int \tan \theta \sec^2 \theta d\theta - \int \tan \theta d\theta$$

    You can now either set $u$ to $\tan \theta$ or $\sec \theta$

    $$u=\tan \theta$$
    $$du=\sec^2 \theta d\theta$$
    $$=\biggl[\frac{1}{2}\tan^2 \theta - -\ln \left|\cos \theta\right|\biggr]^{\frac{\pi}{6}}_{-\frac{\pi}{6}}$$
    $$=\left(\frac{1}{2}\tan^2 \left(\frac{\pi}{6}\right)+\ln \left|\cos \frac{\pi}{6}\right|\right)-\left(\frac{1}{2}\tan^2 \left(-\frac{\pi}{6}\right)+\ln \left|\cos -\frac{\pi}{6}\right|\right)$$
    $$=\frac{1}{2}\left(\frac{1}{\sqrt{3}}\right)^2+\ln \frac{\sqrt{3}}{2}-\frac{1}{2}\left(-\frac{1}{\sqrt{3}}\right)^2-\ln\frac{\sqrt{3}}{2}$$
    $$=\frac{1}{6}+\ln \frac{\sqrt{3}}{2}-\frac{1}{6}-\ln \frac{\sqrt{3}}{2}=0$$
}

\qs{}{
    $$\int^{a}_{0} x\sqrt{x^2+a^2}dx$$
    $$u = x^2+a^2$$
    $$du=2xdx$$
    $$\frac{1}{2}du=xdx$$
    $$=\frac{1}{2}\int u^{\frac{1}{2}}du$$
    $$=\frac{1}{2}\frac{2}{3}u^{\frac{3}{2}}$$
    $$\biggl[\frac{1}{3}\left(x^2+a^2\right)^{\frac{3}{2}}\biggr]^a_0=\frac{1}{3}\left(\left(2a^2\right)^{\frac{3}{2}}-\left(a^2\right)^{\frac{3}{2}}\right)$$
    $$=\frac{1}{3}\left(2\sqrt{2}a^3-a^3\right)$$
}

\nt{
    If the constant is at the top and the variable is at the bottom, you can just swap them and put a negative out front
}

\section*{Exponential integrals}

\dfn{Integrals of exponentials}{
    $$e^u=e^udu\to\int e^udu=e^u+c$$
    $$\ln u = \frac{1}{u}du\to\int \frac{1}{u}du=\ln u + c$$
}

\ex{}{
    $$\int x^2e^{x^3}dx$$
    $$u=x^3$$
    $$du=3x^2dx$$
    $$\frac{1}{3}du=x^2dx$$
    $$\frac{1}{3}\int e^udu$$
    $$\frac{1}{3}e^{x^3}+c$$
}

\ex{}{
    $$\int \frac{x}{x^2+1}dx$$
    $$u=x^2+1$$
    $$du=2xdx$$
    $$\frac{1}{2}du=xdx$$
    $$\frac{1}{2}\int u^{-1}du$$
    $$\frac{1}{2}\int \frac{1}{u}du=\frac{1}{2}\ln \lvert x^2+1\rvert + c$$
}

\ex{}{
    $$\int \tan x dx=\int \frac{\sin x}{\cos x}dx$$
    $$u=\cos x$$
    $$du=-\sin x dx$$
    $$-\int \frac{1}{u}du$$
    $$-\ln \lvert \cos x \rvert + c$$
    $$=\ln \lvert\cos x\rvert^{-1}+c$$
    $$=\ln \lvert \frac{1}{\cos x}\rvert + c$$
    $$=\ln \lvert\sec x\rvert+c$$
}

\qs{}{
    $$\int \left(e^x+e^{-x}\right)^2dx=$$
    $$\int \left(e^{2x}+2+e^{-2x}\right)dx$$
    $$u_1=2x, du_1=2dx, dx=\frac{1}{2}du_1$$
    $$u_2=-2x, du_2=-2dx, dx=\frac{-1}{2}du_2$$
    $$\frac{1}{2}\int e^udu + 2\int dx + \frac{-1}{2}\int e^u du$$
    $$\frac{1}{2}e^{2x}+2x-\frac{1}{2}e^{-2x}+c$$
}

\qs{}{
    $$\int \frac{e^{\frac{1}{x}}}{x^2}dx$$
    $$u=\frac{1}{x}=x^{-1}$$
    $$du=-x^{-2}dx=\frac{-1}{x^2}dx$$
    $$-du=\frac{1}{x^2}dx$$
    $$-\int e^udu$$
    $$-e^{\frac{1}{x}}+c$$
}

\qs{}{
    $$\int \frac{e^{\sqrt{x}}}{\sqrt{x}}$$
    $$u=\sqrt{x}=x^{\frac{1}{2}}$$
    $$du=\frac{1}{2}x^{-\frac{1}{2}}dx=\frac{1}{2}\cdot\frac{1}{\sqrt{x}}dx$$
    $$2du=\frac{1}{\sqrt{x}}dx$$
    $$2\int e^udu$$
    $$2e^{\sqrt{x}}+c$$
}

\qs{}{
    $$\int e^x \sin(e^x)dx$$
    $$u=e^x$$
    $$du=e^xdx$$
    $$\int \sin(u)du$$
    $$-\cos\left(e^x\right) + c$$
}

\qs{}{
    $$\int \frac{\sin 2x}{1+\cos^2 x}dx$$
    $$u = 1+\cos^2 x$$
    $$du=-2\cos(x)\sin(x)dx$$
    $$-du=2\sin(x)\cos(x)=\sin 2x dx$$
    $$-\int \frac{\sin 2x}{u}du$$
    $$-\int \frac{1}{u}du=-\ln \lvert 1+\cos^2 x\rvert+c$$
}